.

src/Hoare.v
@@ -1,10 +1,11 @@
 Require Export imp_state.
 Require Export imp.
+Require Import FunctionalExtensionality.
 
-Definition Assertion := program -> state -> Prop.
+Definition Assertion := state -> Prop.
 
 Definition assert_implies (P Q : Assertion) : Prop :=
-  forall program st, P program st -> Q program st.
+  forall st, P st -> Q st.
 
 Notation "P ->> Q" :=
   (assert_implies P Q) (at level 80) : hoare_spec_scope.
@@ -12,14 +13,329 @@ Open Scope hoare_spec_scope.
 
 Notation "P <<->> Q" :=
   (P ->> Q /\ Q ->> P) (at level 80) : hoare_spec_scope.
+
+Definition assn_sub X a P : Assertion :=
+  fun (st : state) =>
+    P (update st X (aeval st a)).
+     
+Notation "P [ X |-> a ]" := (assn_sub X a P) (at level 10).
+
+Definition assn_sub_list' xs axs P : Assertion :=
+  fun (st : state) =>
+    let st' := zip_state st st xs axs in
+    P st'.
   
 Definition hoare_triple
-           (P:Assertion) (c:com) (Q:Assertion) : Prop :=
-  forall program s st st',
-       c / st || s / st'  ->
-       P program st  ->
-       Q program st'.
+           (P:Assertion) (c:com) (Q:Assertion) : program -> Prop :=
+  fun program =>
+    forall st st' s,
+       c ; program / st || s / st'  ->
+       P st  ->
+       Q st'.
 
 Notation "{{ P }}  c  {{ Q }}" :=
   (hoare_triple P c Q) (at level 90, c at next level)
   : hoare_spec_scope.
+  
+Theorem hoare_consequence_pre : forall (P P' Q : Assertion) c env,
+  {{P'}} c {{Q}} env ->
+  P ->> P' ->
+  {{P}} c {{Q}} env.
+Proof.
+  intros P P' Q c E Hhoare Himp.
+  intros st st' s Hc HP. apply (Hhoare st st' s).
+  assumption. apply Himp. assumption.
+Qed.
+
+Theorem hoare_consequence_post : forall (P Q Q' : Assertion) c env,
+  {{P}} c {{Q'}} env ->
+  Q' ->> Q ->
+  {{P}} c {{Q}} env.
+Proof.
+  intros P Q Q' c env Hhoare Himp.
+  intros st st' s' Hc HP.
+  apply Himp.
+  apply (Hhoare st st' s'); assumption.
+Qed.
+
+Fixpoint ls_disjoint (xs : list id) ys : Prop :=
+	match xs with
+	| x::xs' =>
+	    False = (List.Exists (fun y => y = x) ys)
+	    /\
+	    ls_disjoint xs' ys
+	| nil => True
+	end.
+	
+Lemma update_retrieve : forall st X v,
+  update st X v X = v.
+Proof.
+  intros.
+  unfold update.
+  destruct eq_id_dec; [ reflexivity | congruence].
+Qed.
+
+Lemma update_retrieve_eq : forall st X v v',
+  v = v' ->
+  update st X v X = v'.
+Proof.
+  intros.
+  unfold update.
+  destruct eq_id_dec; [ assumption | congruence].
+Qed.
+
+Lemma update_retrieve_dif : forall st X Y v,
+  X <> Y ->
+  update st X v Y = st Y.
+Proof.
+  intros.
+  unfold update.
+  destruct eq_id_dec; [ congruence | reflexivity ].
+Qed.
+  
+(*** Call ***)
+Theorem hoare_call : forall (program : program) f X args P Q body params rexp r,
+	program f = (body,params,rexp) ->
+	{{ P }}
+	  body
+	{{ fun st => Q st /\ r = aeval st rexp }} program ->
+	{{ fun st => P (zip_state st empty_state params args) }}
+	  CCall f X args
+    {{ fun st => st X = r }} program
+	.
+Proof.
+  unfold hoare_triple.
+  intros.
+  inversion H1; rewrite H6 in H; inversion H; subst.
+  remember (update st X (aeval st'' rexp)) as st'''.
+  specialize (H0 _ _ _ H16 H2).
+  destruct H0.
+  subst.
+  rewrite update_retrieve.
+  reflexivity.
+Qed.
+
+(*** ASSIGNMENT ***)
+
+Theorem hoare_asgn : forall Q X a env,
+  {{Q [X |-> a]}} (X ::= a) {{ Q }} env.
+Proof.
+  unfold hoare_triple.
+  intros.
+  inversion H ; subst.
+  unfold assn_sub in H0.
+  assumption.
+Qed.
+
+(*** IF THEN ELSE ***)
+
+Definition bassn b : Assertion :=
+  fun st => (beval st b = true).
+Lemma bexp_eval_true : forall b st,
+  beval st b = true -> (bassn b) st.
+Proof.
+  intros b st Hbe.
+  unfold bassn. assumption.
+Qed.
+Lemma bexp_eval_false : forall b st,
+  beval st b = false -> ~ ((bassn b) st).
+Proof.
+  intros b st Hbe contra.
+  unfold bassn in contra.
+  rewrite -> contra in Hbe. inversion Hbe.
+Qed.
+
+Theorem hoare_if : forall (P Q : Assertion)  b c1 c2 env,
+  {{fun st => P st /\ bassn b st}} c1 {{Q}} env ->
+  {{fun st => P st /\ ~(bassn b st)}} c2 {{Q}} env ->
+  {{P}} IFB b THEN c1 ELSE c2 FI {{Q}} env.
+Proof.
+  intros.
+  intros st st' s Hc HP.
+  inversion Hc; subst.
+  Case "If true".
+    apply (H st st' s).
+    assumption. split. assumption.
+    apply bexp_eval_true. assumption.
+  Case "If false".
+    apply (H0 st st' s).
+    assumption. split. assumption.
+    apply bexp_eval_false. assumption.
+Qed.
+
+(*******************
+ * EXAMPLE 1       *
+ *******************)
+
+Definition body : com := 
+  Y ::= APlus (AId X) (ANum 1).
+  
+Definition env : program :=
+  fun id =>
+    if eq_id_dec F id
+    then (body, [X], (APlus (AId X) (ANum 1)))
+    else (CSkip, [], ANum 0)
+    .
+
+Lemma body_p : forall Q X Y,
+  Q = (fun st => st Y = st X + 1) ->
+  {{ Q[Y |-> (APlus (AId X) (ANum 1))] }}
+    Y ::= APlus (AId X) (ANum 1)
+  {{ Q }} env.
+Proof.
+  intros Q X Y H.
+  rewrite H.
+  apply hoare_asgn.
+Qed.
+
+Theorem prog_correct :
+  {{fun st => True}}
+    CCall F Z [ANum 2]
+  {{fun st => st Z = 3}} env.
+Proof.
+  eapply hoare_consequence_pre.
+  apply hoare_call with (params := [X]) (Q := fun st => st Y = 3)
+                  (body := body) (rexp := (APlus (AId X) (ANum 1))).
+  unfold env. simpl. reflexivity.
+  apply hoare_asgn.
+  intro. intros _.
+  unfold assn_sub.
+  simpl.
+  split; try rewrite update_retrieve; reflexivity.
+Qed.
+
+(*******************
+ * EXAMPLE 2       *
+ ******************* )
+
+Definition Fbody : com := 
+  IFB (BEq (ANum 0) (AId X))
+  THEN Z ::= APlus (AId Y) (ANum 1)
+  ELSE CCall G Z [AId Y]
+  FI.
+  
+Definition Gbody : com := 
+  Z ::= APlus (AId Y) (ANum 1) ;;
+  Z ::= APlus (AId Z) (ANum 1)
+  .
+  
+Definition env'' : program :=
+  fun id =>
+    if eq_id_dec F id
+    then (Fbody, cons X (cons Y nil), (APlus (AId X) (AId Y)))
+    else if eq_id_dec G id
+    then (Gbody, [X], (APlus (AId X) (ANum 2)))
+    else (CSkip, [], ANum 0)  
+  .
+  
+Theorem prog_correct'' :
+  {{fun st => True}}
+    CCall F Z (cons (ANum 10) (cons (ANum 10) nil))
+  {{fun st => st Z = 20}} env''.
+Proof.
+  eapply hoare_consequence_pre.
+  apply hoare_call with (params := cons X (cons Y nil))
+			      (Q := fun st => st Z = st X + st Y)
+                  (body := Fbody) (rexp := (APlus (AId X) (AId Y)))
+                  (P := fun st => st X + st Y = st X + st Y /\ st X = 10 /\ st Y = 10).
+  unfold env''. simpl. reflexivity.
+  eapply hoare_consequence_post with (Q' := fun st => st Z = st X + st Y /\ st X = 10 /\ st Y = 10).
+  eapply hoare_consequence_pre with (P' := fun st => True).
+  unfold body''.
+  apply b''.
+  intro; intros; apply I.
+  intro; intros.
+  destruct H.
+  split. assumption.
+  unfold aeval. destruct H0; rewrite H0, H1; reflexivity.
+  intros st _. simpl.
+  split. reflexivity.
+  rewrite update_retrieve_dif, update_retrieve, update_retrieve.
+  split; reflexivity.
+  unfold Y, X, not; intro; congruence.
+Qed. *)
+
+Definition body'' : com := 
+  IFB (BEq (ANum 1) (AId X))
+  THEN Z ::= APlus (AId Y) (AId X)
+  ELSE CCall F Z (cons (AMinus (AId X) (ANum 1))
+				   (cons (APlus (AId Y) (ANum 1))
+ 					 nil))
+  FI.
+(*  
+Definition env'' : program :=
+  fun id =>
+    if eq_id_dec F id
+    then (body'', cons X (cons Y nil), (APlus (AId X) (AId Y)))
+    else (CSkip, [], ANum 0)
+    .
+
+( * 
+  {{ fun st => st X > 0 }} env
+  IFB (BEq (ANum 1) (AId X)) THEN
+    {{ fun st => st X = 1 /\ st X + Y = st X + Y }} env ->>
+    {{ fun st => st X + Y = st X + Y }} env
+    Z ::= APlus (AId X) (AId Y)
+    {{ fun st => st Z = st X + Y }} env
+  ELSE
+    {{ fun st => st X > 1 /\ st X + st Y = st X + st Y }} env
+    CCall F Z (cons (AMinus (AId X) (ANum 1))
+		   		 (cons (APlus (AId Y) (ANum 1))
+ 					nil))
+ 	{{ fun st => st X > 1 /\ st Z = st X + st Y }} env ->>
+ 	{{ fun st => st Z = st X + st Y }} env
+  FI.
+  {{ fun st => st Z = st X + st Y }} env * )
+
+Lemma b'' : forall X Y Z x y z env,
+  z = x + y ->
+  {{ (fun st => z = st Z /\ x = st X /\ y = st Y)[Z |-> APlus (AId Y) (AId X)] }}
+  IFB (BEq (ANum 1) (AId X))
+  THEN Z ::= APlus (AId Y) (AId X)
+  ELSE CCall F Z (cons (AMinus (AId X) (ANum 1))
+				   (cons (APlus (AId Y) (ANum 1))
+ 					 nil))
+  FI
+  {{ fun st => st Z = st X + st Y }} env.
+Proof.
+  intros X Y Z x y z env H.
+  apply hoare_if.
+  eapply hoare_consequence_post
+	with (Q' := fun st : state => st Z = st X + st Y).
+  eapply hoare_consequence_pre.
+  eapply hoare_asgn.
+  intro. intros.
+  unfold assn_sub in *.
+  destruct H0; destruct H0; destruct H2.
+  rewrite <- H0; rewrite <- H2; rewrite <- H3.
+  assumption.
+  intro; intros.
+  assumption.
+Admitted.
+
+Theorem prog_correct'' :
+  {{fun st => True}}
+    CCall F Z (cons (ANum 10) (cons (ANum 10) nil))
+  {{fun st => st Z = 20}} env''.
+Proof.
+  eapply hoare_consequence_pre.
+  apply call with (params := cons X (cons Y nil))
+			      (Q := fun st => st Z = st X + st Y)
+                  (body := body'') (rexp := (APlus (AId X) (AId Y)))
+                  (P := fun st => st X + st Y = st X + st Y /\ st X = 10 /\ st Y = 10).
+  unfold env''. simpl. reflexivity.
+  eapply hoare_consequence_post with (Q' := fun st => st Z = st X + st Y /\ st X = 10 /\ st Y = 10).
+  eapply hoare_consequence_pre with (P' := fun st => True).
+  unfold body''.
+  apply b''.
+  intro; intros; apply I.
+  intro; intros.
+  destruct H.
+  split. assumption.
+  unfold aeval. destruct H0; rewrite H0, H1; reflexivity.
+  intros st _. simpl.
+  split. reflexivity.
+  rewrite update_retrieve_dif, update_retrieve, update_retrieve.
+  split; reflexivity.
+  unfold Y, X, not; intro; congruence.
+Qed. *)
