src/imp.v
@@ -1,5 +1,4 @@
 Require Export imp_state.
-Require Export Logic.
 
 Definition X : id := Id 0.
 Definition Y : id := Id 1.
@@ -36,65 +35,191 @@ Fixpoint beval (st : state) (b : bexp) : bool :=
       negb (beval st b1)
   | BAnd b1 b2  =>
       andb (beval st b1) (beval st b2)
-  end.  
+  end.   
   
-Fixpoint zip_state (st : state) (ids : list id) (vs : list nat) : state :=
+Fixpoint zip_state (steval st : state) (ids : list id) (vs : list aexp) : state :=
   match ids with
   | i::ids' => 
   	match vs with
   	| v::vs' =>
-  		let st' := update st i v in
-  		zip_state st' ids' vs'
+  		let st' := update st i (aeval steval v) in
+  		zip_state steval st' ids' vs'
   	| [] => st
   	end
   | [] => st
   end.
 
-Reserved Notation "c1 '/' st '||' s '/' st'"
-                  (at level 40, st, s at level 39).
+Fixpoint assigned_vars (c : com) (vars : list id): list id :=
+	match c with
+	| CAss i _ =>
+		i::vars
+	| CSeq c1 c2
+	| CIf _ c1 c2 =>
+		let vars' := assigned_vars c1 vars in
+		assigned_vars c2 vars'
+	| CWhile _ c' =>
+		assigned_vars c' vars
+	| _ => vars
+	end.
   
-Inductive ceval' : com -> state -> status -> state -> Prop :=
-  | E_Skip : forall st,
-      CSkip / st || SContinue / st
-  | E_Break: forall st,
-      CBreak / st || SBreak / st
-  | E_Ass : forall st st' ident a n,
+Inductive ls_disjoint : list id -> list id -> Prop :=
+  | LSD_n: forall ys, ls_disjoint [] ys
+  | LSD_S: forall x xs ys, ls_disjoint xs ys ->
+              not (Exists (fun x' => x = x') ys) -> 
+              ls_disjoint (x::xs) ys.
+  
+Lemma zip_state_tr : forall steval st st' p q ids r s vs,
+  p <> q ->
+  st = zip_state steval st' (p::q::ids) (r::s::vs) ->
+  st = zip_state steval st' (q::p::ids) (s::r::vs).
+Proof.
+  intros.
+  unfold zip_state. fold zip_state.
+  unfold zip_state in H1. fold zip_state in H1.
+Admitted.
+
+Inductive entry_state : state -> state -> list id -> list aexp -> Prop :=
+  | ES_n: forall steval, entry_state steval empty_state nil nil
+  | ES_S: forall steval st p ps v vs,
+  			entry_state steval st ps vs ->
+  			entry_state steval (update st p (aeval steval v)) (p::ps) (v::vs).
+  
+Inductive list_unique_items {T : Type} : (list T) -> Prop :=
+  | LUI_n: list_unique_items []
+  | LUI_S: forall xs x, Exists (fun x' => x = x') xs = False -> list_unique_items (x::xs). 
+
+Reserved Notation "c1 ';' program '/' st '||' s '/' st'"
+                  (at level 40, program, st, s at level 39).
+  
+Inductive ceval : com -> program -> state -> status -> state -> Prop :=
+  | E_Skip : forall st program,
+      CSkip ; program / st || SContinue / st
+  | E_Break: forall st program,
+      CBreak ; program / st || SBreak / st
+  | E_Ass : forall st st' ident a n program,
       aeval st a = n ->
       update st ident n = st' ->
-      CAss ident a / st || SContinue / st'
-  | E_If_True : forall st st' b status c1 c2,
+      CAss ident a ; program / st || SContinue / st'
+  | E_If_True : forall st st' b status c1 c2 program,
       beval st b = true ->
-      c1 / st || status / st' ->
-      CIf b c1 c2 / st || status / st'
-  | E_If_False : forall st st' b status c1 c2,
+      c1 ; program / st || status / st' ->
+      CIf b c1 c2 ; program / st || status / st'
+  | E_If_False : forall st st' b status c1 c2 program,
       beval st b = false ->
-      c2 / st || status / st' ->
-      CIf b c1 c2 / st || status / st'
-  | E_Seq : forall st st' st'' c1 c2 status,
-      c1 / st || SContinue / st' ->
-      c2 / st' || status / st'' ->
-      CSeq c1 c2 / st || status / st''
-  | E_Seq_Break : forall st st' c1 c2,
-      c1 / st || SBreak / st' ->
-      CSeq c1 c2 / st || SBreak / st'
-  | E_While_Break : forall st st' b c,
+      c2 ; program / st || status / st' ->
+      CIf b c1 c2 ; program / st || status / st'
+  | E_Seq : forall st st' st'' c1 c2 status program,
+      c1 ; program / st || SContinue / st' ->
+      c2 ; program / st' || status / st'' ->
+      CSeq c1 c2 ; program / st || status / st''
+  | E_Seq_Break : forall st st' c1 c2 program,
+      c1 ; program / st || SBreak / st' ->
+      CSeq c1 c2 ; program / st || SBreak / st'
+  | E_While_Break : forall st st' b c program,
       beval st b = true ->
-      c / st || SBreak / st' ->
-      CWhile b c / st || SContinue / st'
-  | E_While_False : forall st b c,
+      c ; program / st || SBreak / st' ->
+      CWhile b c ; program / st || SContinue / st'
+  | E_While_False : forall st b c program,
       beval st b = false ->
-      CWhile b c / st || SContinue / st
-  | E_While_True : forall st st' st'' b c,
+      CWhile b c ; program / st || SContinue / st
+  | E_While_True : forall st st' st'' b c program,
       beval st b = true ->
-      c / st || SContinue / st' ->
-      CWhile b c / st' || SContinue / st'' ->
-      CWhile b c / st || SContinue / st''
-  | E_Call : forall st st' st'' ident status p program c rexp params args entry_st,
+      c ; program / st || SContinue / st' ->
+      CWhile b c ; program / st' || SContinue / st'' ->
+      CWhile b c ; program / st || SContinue / st''
+  | E_Call : forall st st' st'' entry_st status f program body params args X rexp,
+      program f = (body, params, rexp) ->
+      list_unique_items params ->
+      list_unique_items args ->
+      length params = length args ->
+      ls_disjoint params (assigned_vars body []) ->
+      entry_st = zip_state st empty_state params args -> 
+      body ; program / entry_st || status / st'' ->
+      st' = update st X (aeval st'' rexp) ->
+      CCall f X args ; program / st || SContinue / st'
+     
+  (* | E_Call : forall st st' st'' entry_st status f program body params args X rexp,
+      program f = (body, params, rexp) ->
+      entry_st = update empty_state params (aeval st args) -> 
+      body ; program / entry_st || status / st'' ->
+      st' = update st X (aeval st'' rexp) ->
+      CCall f X args ; program / st || SContinue / st' *)
+      
+  (*| E_Call : forall st st' status f program body params args X rexp,
+      program f = (body, params, rexp) ->
+      body ; program / st || status / st' ->
+      CCall f X args ; program / st || SContinue / st' *)
+      
+  (*| E_Call : forall st st' st'' ident status p program c rexp params args entry_st x,
       program p = (c, params, rexp) ->
       length params = length args ->
-      entry_st = zip_state empty_state params args ->
+      entry_st = update st params args ->
       c / entry_st || status / st ->
-      st'' = update st' ident (aeval st rexp) ->
-      CCall ident p args / st' || SContinue / st''
+      x = aeval st rexp ->
+      st'' = update st' ident x ->
+      CCall ident p args / st' || SContinue / st'' *)
 
-  where "c1 '/' st '||' s '/' st'" := (ceval' c1 st s st').
+  where "c1 ';' program '/' st '||' s '/' st'" := (ceval c1 program st s st').
+  
+(*Theorem ceval_deterministic: forall (c:com) st st1 st2 s1 s2,
+     c / st || s1 / st1  ->
+     c / st || s2 / st2 ->
+     st1 = st2 /\ s1 = s2.
+Proof.
+  intros.
+  generalize dependent s2.
+  generalize dependent st2.
+  induction H0; intros.
+  Case "E_Skip". inversion H1; subst; split; reflexivity.
+  Case "E_Break". inversion H1; subst; split; reflexivity.
+  Case "E_Ass". inversion H2; subst; split; reflexivity.
+  Case "E_If_True".
+    inversion H2; subst.
+    apply IHceval', H10.
+    rewrite H0 in H9; inversion H9.
+  Case "E_If_False".
+    inversion H2; subst.
+    rewrite H0 in H9; inversion H9.
+    apply IHceval'; apply H10.
+  Case "E_Seq".
+    inversion H1; subst.
+    specialize (IHceval'1 _ _ H3).
+    destruct IHceval'1; subst.    
+    apply IHceval'2, H7.
+    specialize (IHceval'1 _ _ H6).
+    destruct IHceval'1.
+    congruence.
+  Case "E_Seq_Break".
+    inversion H1; subst.
+    specialize (IHceval' _ _ H4); subst.
+    destruct IHceval'.
+    congruence.
+    apply IHceval'.
+    assumption.
+  Case "E_While_Break".
+    inversion H2; subst.
+    specialize (IHceval' _ _ H9).
+    destruct IHceval'.
+    split; [ assumption | reflexivity ].
+    congruence.
+    specialize (IHceval' _ _ H6).
+    destruct IHceval'.
+    congruence.
+  Case "E_While_False".
+    inversion H1; subst.
+    congruence.
+    split; reflexivity.
+    congruence.
+  Case "E_While_True".
+    inversion H1; subst.
+    specialize (IHceval'1 _ _ H8).
+    destruct IHceval'1.
+    congruence.
+    congruence.
+    specialize (IHceval'1 _ _ H5); destruct IHceval'1; subst.
+    specialize (IHceval'2 _ _ H9); assumption. 
+  Case "E_Call".
+    inversion H6; subst.
+    specialize (IHceval' _ _ H3).
+    subst.
+Qed.*)
