src/imp_state.v
@@ -2,7 +2,7 @@ Require Export imp_ast.
 
 Definition state := id -> nat.
 
-Definition program := id -> com.
+Definition program := id -> com * list  id * aexp.
 
 Inductive status : Type :=
   | SContinue : status
